pulse/share/pulse/examples/dice/dpe/DPETypes.fsti
@@ -281,22 +281,46 @@ let context_perm (context:context_t) (repr:context_repr_t): vprop =
   | L1_context c, L1_context_repr r -> l1_context_perm c r
   | _ -> pure False
 
+let context_and_repr_tag_related (c:context_t) (r:context_repr_t) : bool =
+  match c, r with
+  | Engine_context _, Engine_context_repr _
+  | L0_context _, L0_context_repr _
+  | L1_context _, L1_context_repr _ -> true
+  | _ -> false
+
 ```pulse
 ghost
-fn rewrite_context_perm_engine (c:engine_context_t) (r:context_repr_t)
-  requires context_perm (Engine_context c) r
+fn intro_context_and_repr_tag_related (c:context_t) (r:context_repr_t)
+  requires context_perm c r
+  ensures context_perm c r ** pure (context_and_repr_tag_related c r)
+{
+  let b = context_and_repr_tag_related c r;
+  if b {
+    ()
+  } else {
+    rewrite (context_perm c r) as (pure False);
+    unreachable ()
+  }
+}
+```
+
+```pulse
+ghost
+fn rewrite_context_perm_engine (c:context_t) (ec:engine_context_t) (#r:context_repr_t)
+  requires context_perm c r **
+           pure (c == Engine_context ec)
   returns uds:Ghost.erased (Seq.seq U8.t)
-  ensures engine_context_perm c uds ** pure (r == Engine_context_repr uds)
+  ensures engine_context_perm ec uds ** pure (r == Engine_context_repr uds)
 {
   match r {
     Engine_context_repr uds -> {
-      rewrite (context_perm (Engine_context c) r) as
-              (engine_context_perm c uds);
+      rewrite (context_perm c r) as
+              (engine_context_perm ec uds);
       hide uds
     }
     _ -> {
       assume_ (pure (~ (Engine_context_repr? r)));
-      rewrite (context_perm (Engine_context c) r) as
+      rewrite (context_perm c r) as
               (pure False);
       unreachable ()
 
@@ -307,20 +331,21 @@ fn rewrite_context_perm_engine (c:engine_context_t) (r:context_repr_t)
 
 ```pulse
 ghost
-fn rewrite_context_perm_l0 (c:l0_context_t) (r:context_repr_t)
-  requires context_perm (L0_context c) r
-  returns r1:Ghost.erased l0_context_repr_t
-  ensures l0_context_perm c r1 ** pure (r == L0_context_repr r1)
+fn rewrite_context_perm_l0 (c:context_t) (lc:l0_context_t) (#r:context_repr_t)
+  requires context_perm c r **
+           pure (c == L0_context lc)
+  returns lrepr:Ghost.erased l0_context_repr_t
+  ensures l0_context_perm lc lrepr ** pure (r == L0_context_repr lrepr)
 {
   match r {
-    L0_context_repr r1 -> {
-      rewrite (context_perm (L0_context c) r) as
-              (l0_context_perm c r1);
-      hide r1
+    L0_context_repr lrepr -> {
+      rewrite (context_perm c r) as
+              (l0_context_perm lc lrepr);
+      hide lrepr
     }
     _ -> {
       assume_ (pure (~ (L0_context_repr? r)));
-      rewrite (context_perm (L0_context c) r) as
+      rewrite (context_perm c r) as
               (pure False);
       unreachable ()
     }
@@ -330,20 +355,21 @@ fn rewrite_context_perm_l0 (c:l0_context_t) (r:context_repr_t)
 
 ```pulse
 ghost
-fn rewrite_context_perm_l1 (c:l1_context_t) (r:context_repr_t)
-  requires context_perm (L1_context c) r
-  returns r1:Ghost.erased l1_context_repr_t
-  ensures l1_context_perm c r1 ** pure (r == L1_context_repr r1)
+fn rewrite_context_perm_l1 (c:context_t) (lc:l1_context_t) (#r:context_repr_t)
+  requires context_perm c r **
+           pure (c == L1_context lc)
+  returns lrepr:Ghost.erased l1_context_repr_t
+  ensures l1_context_perm lc lrepr ** pure (r == L1_context_repr lrepr)
 {
   match r {
-    L1_context_repr r1 -> {
-      rewrite (context_perm (L1_context c) r) as
-              (l1_context_perm c r1);
-      hide r1
+    L1_context_repr lrepr -> {
+      rewrite (context_perm c r) as
+              (l1_context_perm lc lrepr);
+      hide lrepr
     }
     _ -> {
       assume_ (pure (~ (L1_context_repr? r)));
-      rewrite (context_perm (L1_context c) r) as
+      rewrite (context_perm c r) as
               (pure False);
       unreachable ()
     }
@@ -378,19 +404,20 @@ let record_perm (record:record_t) (p:perm) (repr:repr_t)  : vprop =
 
 ```pulse
 ghost
-fn rewrite_record_perm_engine (r:engine_record_t) (p:perm) (repr:repr_t)
-  requires record_perm (Engine_record r) p repr
-  returns r0:Ghost.erased engine_record_repr
-  ensures engine_record_perm r p r0 ** pure (repr == Engine_repr r0)
+fn rewrite_record_perm_engine (r:record_t) (er:engine_record_t) (#p:perm) (#repr:repr_t)
+  requires record_perm r p repr **
+           pure (r == Engine_record er)
+  returns erepr:Ghost.erased engine_record_repr
+  ensures engine_record_perm er p erepr ** pure (repr == Engine_repr erepr)
 {
   match repr {
-    Engine_repr r0 -> {
-      rewrite (record_perm (Engine_record r) p repr)
-          as  (engine_record_perm r p r0);
-      hide r0
+    Engine_repr erepr -> {
+      rewrite (record_perm r p repr)
+          as  (engine_record_perm er p erepr);
+      hide erepr
     }
     L0_repr _ -> {
-      rewrite (record_perm (Engine_record r) p repr)
+      rewrite (record_perm r p repr)
           as  (pure False);
       unreachable ()
     }
@@ -400,20 +427,21 @@ fn rewrite_record_perm_engine (r:engine_record_t) (p:perm) (repr:repr_t)
 
 ```pulse
 ghost
-fn rewrite_record_perm_l0 (r:l0_record_t) (p:perm) (repr:repr_t)
-  requires record_perm (L0_record r) p repr
+fn rewrite_record_perm_l0 (r:record_t) (lr:l0_record_t) (#p:perm) (#repr:repr_t)
+  requires record_perm r p repr **
+           pure (r == L0_record lr)
   returns r0:Ghost.erased l0_record_repr_t
-  ensures l0_record_perm r p r0 ** pure (repr == L0_repr r0)
+  ensures l0_record_perm lr p r0 ** pure (repr == L0_repr r0)
 {
   match repr {
     Engine_repr _ -> {
-      rewrite (record_perm (L0_record r) p repr)
+      rewrite (record_perm r p repr)
           as  (pure False);
       unreachable ()
     }
     L0_repr r0 -> {
-      rewrite (record_perm (L0_record r) p repr)
-          as  (l0_record_perm r p r0);
+      rewrite (record_perm r p repr)
+          as  (l0_record_perm lr p r0);
       hide r0
     }
   }
